src/PlutusIR/Semantics/TypeSafety/BaseKindedness.v
@@ -2,7 +2,8 @@ Require Import PlutusCert.PlutusIR.
 Require Import PlutusCert.PlutusIR.Semantics.Static.
 Require Import PlutusCert.PlutusIR.Semantics.TypeSafety.TypeLanguage.Preservation.
 Require Import PlutusCert.PlutusIR.Semantics.TypeSafety.TypeLanguage.StrongNormalisation.
-Require Import PlutusCert.PlutusIR.Semantics.TypeSafety.SubstitutionPreservesTyping.
+
+Require Import PlutusCert.PlutusIR.Semantics.TypeSafety.SubstitutionPreservesTyping.SubstituteTCA.
 
 Ltac solver := try solve [repeat (econstructor; eauto)].
 
