src/PlutusIR/Semantics/TypeSafety/TypeLanguage/StrongNormalisation.v
@@ -1,6 +1,6 @@
 Require Import PlutusCert.PlutusIR.Semantics.Static.
 Require Import PlutusCert.PlutusIR.Semantics.Dynamic.
-Require Import PlutusCert.PlutusIR.Semantics.TypeSafety.SubstitutionPreservesTyping.
+Require Import PlutusCert.PlutusIR.Semantics.TypeSafety.SubstitutionPreservesTyping.TypeSubstitution.
 
 Theorem strong_normalisation : forall Delta T K,
     Delta |-* T : K ->
